Propagate changes to code

code/blake2/Hacl.Impl.Blake2.Core.fst
@@ -31,7 +31,10 @@ let row_v #a #m h r =
 
 let row_v_lemma #a #m h0 h1 r1 r2 = ()
 
-let create_default_params a salt personal = {
+let alloca_default_params a =
+  let salt = create (salt_len a) (u8 0) in
+  let personal = create (personal_len a) (u8 0) in
+  {
       digest_length = u8 32;
       key_length = u8 0;
       fanout = u8 1;
