code/streaming/Hacl.Streaming.Blake2.Common.fst
@@ -172,7 +172,7 @@ let unit_to_stateful_key_t (a : alg):
   Tot (stateful_key_t a false 0) =
   ((), ())
 
-#push-options "--z3rlimit 100"
+#push-options "--z3rlimit 100 --ifuel 1"
 
 /// The ``has_key`` parameter is meta
 /// TODO: this definition could be moved to Hacl.Streaming.Interface, it could
